reify ack into STLC+NatRec using string names

Contender.v
@@ -19,6 +19,335 @@ Fixpoint ack (n a b : nat) :=
 (* Submitted by codyroux *)
 Definition contender_4 := ack 5 42 10002.
 
+
+Definition ack'(n: nat): nat -> nat -> nat :=
+  Nat.recursion
+    (fun a b => S b)
+    (fun (pred0: nat) (rec0: nat -> nat -> nat) =>
+       Nat.recursion
+         (Nat.recursion (fun (m: nat) => m)
+                        (fun (pred: nat) (rec: nat -> nat) (m: nat) => S (rec m)))
+         (fun (pred: nat) (rec: nat -> nat -> nat) =>
+            (fun a b => Nat.recursion 1 (fun pred1 rec1 => rec a rec1) b))
+         pred0)
+    n.
+
+Lemma iter_proper: forall f1 f2,
+    (forall x, f1 x = f2 x) ->
+    forall b, iter f1 b = iter f2 b.
+Proof.
+  induction b.
+  - reflexivity.
+  - simpl. rewrite IHb. apply H.
+Qed.
+
+Definition iter' (f : nat -> nat) : nat -> nat :=
+  Nat.recursion 1 (fun (pred: nat) (rec: nat) => f rec).
+
+Lemma iter'_equiv: forall f b, iter' f b = iter f b.
+Proof. induction b; intros; simpl; congruence. Qed.
+
+Definition add': nat -> nat -> nat :=
+  Nat.recursion (fun (m: nat) => m) (fun (pred: nat) (rec: nat -> nat) (m: nat) => S (rec m)).
+
+Lemma add'_equiv: forall n m, add' n m = Nat.add n m.
+Proof.
+  induction n; intros; simpl.
+  - reflexivity.
+  - rewrite <- IHn. reflexivity.
+Qed.
+
+Lemma ack'_equiv: forall n a b, ack' n a b = ack n a b.
+Proof.
+  induction n; intros; simpl.
+  - reflexivity.
+  - destruct n.
+    + simpl. apply add'_equiv.
+    + specialize (IHn a).
+      rewrite <- (iter_proper _ _ IHn).
+      rewrite <- iter'_equiv. reflexivity.
+Qed.
+
+
+Notation "' x <- a ; f" :=
+  (match (a: option _) with
+   | x => f
+   | _ => None
+   end)
+  (right associativity, at level 70, x pattern).
+
+Inductive type :=
+| tpNat: type
+| tpArr: type -> type -> type.
+
+Fixpoint type_eqb(t1 t2: type): bool :=
+  match t1, t2 with
+  | tpNat, tpNat => true
+  | tpArr A B, tpArr C D => andb (type_eqb A C) (type_eqb B D)
+  | _, _ => false
+  end.
+
+Fixpoint interp_type(tp: type): Type :=
+  match tp with
+  | tpNat => nat
+  | tpArr t1 t2 => (interp_type t1) -> (interp_type t2)
+  end.
+
+Require Import List String.
+
+Inductive term :=
+| tVar(x: string)
+| tLam(x: string)(A B: type)(body: term)
+| tApp(t1 t2: term)
+| tO
+| tS
+| tNatRec(R: type).
+
+Definition lookup{T}(e: list (string * T))(x: string): option T :=
+  'Some (_, t) <- List.find (fun '(y, t) => String.eqb x y) e; Some t.
+
+Definition error{tp: type}: interp_type tp.
+  revert tp.
+  refine (fix rec tp := _).
+  destruct tp; simpl.
+  - exact 42.
+  - intros _. apply rec.
+Defined.
+
+Definition cast_error(from to: type):
+  ((interp_type from -> interp_type to) * (interp_type to -> interp_type from)).
+  split; intros; exact error.
+Qed.
+
+Definition cast_impl(from to: type):
+  ((interp_type from -> interp_type to) * (interp_type to -> interp_type from)).
+  revert from to.
+  induction from; intros; simpl in *.
+  - destruct to; simpl.
+    + split; exact id.
+    + exact (cast_error tpNat (tpArr to1 to2)).
+  - destruct to.
+    + exact (cast_error (tpArr from1 from2) tpNat).
+    + destruct (type_eqb from1 to1) eqn: E1;
+      destruct (type_eqb from2 to2) eqn: E2;
+      simpl in *.
+      {
+        specialize (IHfrom1 to1).
+        specialize (IHfrom2 to2).
+        destruct IHfrom1 as [F1T1 T1F1].
+        destruct IHfrom2 as [F2T2 T2F2].
+        split.
+        * intros F arg. apply F2T2. apply F. apply T1F1. apply arg.
+        * intros F arg. apply T2F2. apply F. apply F1T1. apply arg.
+      }
+      all: exact (cast_error (tpArr from1 from2) (tpArr to1 to2)).
+Defined.
+
+(* designed to be computable (no opaque proofs) *)
+Definition cast{from: type}(to: type): interp_type from -> interp_type to :=
+  fst (cast_impl from to).
+
+Definition interp_term: forall (e: list (string * {tp: type & interp_type tp})) (t: term),
+    {tp: type & interp_type tp}.
+  refine (fix rec e t {struct t} :=
+  match t with
+  | tVar x => _
+  | tLam x A B body => _
+  | tApp t1 t2 => _
+  | tO => _
+  | tS => _
+  | tNatRec R => _
+  end).
+  - destruct (lookup e x) as [R|].
+    + exact R.
+    + exact (existT _ tpNat error).
+  - refine (existT _ (tpArr A B) _).
+    simpl.
+    intro x'.
+    set (r := (projT2 (rec ((x, (existT _ A x')) :: e) body))).
+    simpl in r.
+    exact (cast B r).
+  - destruct (rec e t1) as [R1 r1] eqn: E1.
+    destruct (rec e t2) as [R2 r2] eqn: E2.
+    destruct R1 as [|A B]; [exact (existT _ tpNat error)|].
+    simpl in *.
+    exact (existT _ _ (r1 (cast A r2))).
+  - exact (existT _ tpNat 0).
+  - exact (existT _ (tpArr tpNat tpNat) S).
+  - set (r := (@Nat.recursion (interp_type R))).
+    exact (existT _ (tpArr R (tpArr (tpArr tpNat (tpArr R R)) (tpArr tpNat R))) r).
+Defined.
+
+Definition type_eq_dec: forall x y : type, {x = y} + {x <> y}.
+  induction x; destruct y eqn: E; intros; simpl.
+  - left. reflexivity.
+  - right. intro C. discriminate.
+  - right. intro C. discriminate.
+  - specialize (IHx1 t1).
+    specialize (IHx2 t2).
+    destruct IHx1 as [E1 | N1]; destruct IHx2 as [E2 | N2]; try (right; congruence).
+    left. subst. reflexivity.
+Defined.
+
+Lemma type_eqb_true: forall t1 t2, type_eqb t1 t2 = true -> t1 = t2.
+Proof.
+  induction t1; intros; destruct t2; simpl in *; try congruence.
+  apply Bool.andb_true_iff in H. destruct H. f_equal; eauto.
+Qed.
+
+Lemma type_eqb_same: forall t, type_eqb t t = true.
+Proof.
+  induction t; simpl.
+  - reflexivity.
+  - rewrite IHt1, IHt2. reflexivity.
+Qed.
+
+Require Import FunctionalExtensionality.
+
+Lemma cast_impl_same: forall (B: type) (t: interp_type B),
+    fst (cast_impl B B) t = t /\ snd (cast_impl B B) t = t.
+Proof.
+  induction B; intros; simpl; unfold id.
+  - auto.
+  - do 2 rewrite type_eqb_same.
+    destruct (cast_impl B1 B1) as [fw1 bw1] eqn: E1.
+    destruct (cast_impl B2 B2) as [fw2 bw2] eqn: E2.
+    simpl in *.
+    split; extensionality arg.
+    + specialize (IHB1 arg).
+      apply proj2 in IHB1.
+      rewrite IHB1.
+      specialize (IHB2 (t arg)).
+      apply proj1 in IHB2.
+      exact IHB2.
+    + specialize (IHB1 arg).
+      apply proj1 in IHB1.
+      rewrite IHB1.
+      specialize (IHB2 (t arg)).
+      apply proj2 in IHB2.
+      exact IHB2.
+Qed.
+
+Lemma cast_same: forall (B: type) (t: interp_type B),
+    cast B t = t.
+Proof.
+  intros. unfold cast.
+  pose proof (cast_impl_same B t) as P.
+  apply proj1 in P.
+  exact P.
+Qed.
+
+Lemma interp_tVar: forall e x (p: {tp: type & interp_type tp}),
+    lookup e x = Some p ->
+    interp_term e (tVar x) = p.
+Proof. intros. simpl. rewrite H. reflexivity. Qed.
+
+Lemma interp_tVar_head: forall e x (p: {tp: type & interp_type tp}),
+    interp_term ((x, p) :: e) (tVar x) = p.
+Proof.
+  intros. simpl. unfold lookup, List.find.
+  rewrite String.eqb_refl. reflexivity.
+Qed.
+
+Lemma interp_tVar_tail: forall e x y (p1 p2: {tp: type & interp_type tp}),
+    String.eqb y x = false ->
+    interp_term e (tVar y) = p2 ->
+    interp_term ((x, p1) :: e) (tVar y) = p2.
+Proof.
+  intros. simpl. unfold lookup, List.find.
+  rewrite H. rewrite <- H0. reflexivity.
+Qed.
+
+Lemma interp_tLam: forall e x A B body f,
+  (forall x0, interp_term ((x, existT interp_type A x0) :: e) body = existT _ B (f x0)) ->
+  interp_term e (tLam x A B body) = existT _ (tpArr A B) f.
+Proof.
+  simpl.
+  intros.
+  f_equal.
+  extensionality x'.
+  specialize (H x').
+  destruct (interp_term ((x, existT interp_type A x') :: e) body) eqn: E.
+  inversion H.
+  subst.
+  simpl.
+  apply cast_same.
+Qed.
+
+Lemma interp_tApp: forall e t1 t2 A B (f: interp_type A -> interp_type B) (a: interp_type A),
+    interp_term e t1 = existT _ (tpArr A B) f ->
+    interp_term e t2 = existT _ A a ->
+    interp_term e (tApp t1 t2) = existT _ B (f a).
+Proof.
+  intros.
+  simpl.
+  destruct (interp_term e t1) eqn: E1.
+  destruct (interp_term e t2) eqn: E2.
+  pose proof (EqdepFacts.eq_sigT_fst H). subst x.
+  apply Eqdep_dec.inj_pair2_eq_dec in H. 2: apply type_eq_dec. subst i.
+  pose proof (EqdepFacts.eq_sigT_fst H0). subst x0.
+  apply Eqdep_dec.inj_pair2_eq_dec in H0. 2: apply type_eq_dec. subst i0.
+  rewrite cast_same.
+  reflexivity.
+Qed.
+
+Lemma interp_tO: forall e, interp_term e tO = existT _ tpNat 0.
+Proof. intros. reflexivity. Qed.
+
+Lemma interp_tS: forall e, interp_term e tS = existT _ (tpArr tpNat tpNat) S.
+Proof. intros. reflexivity. Qed.
+
+Lemma interp_tNatRec: forall e R,
+    interp_term e (tNatRec R) =
+    existT _ (tpArr R (tpArr (tpArr tpNat (tpArr R R)) (tpArr tpNat R)))
+           (@Nat.recursion (interp_type R)).
+Proof.
+  intros. subst. reflexivity.
+Qed.
+
+(*
+Notation "A --> B" := (tpArr A B) (at level 60, right associativity).
+*)
+
+Ltac reify_type T :=
+  lazymatch T with
+  | ?A -> ?B => let A' := reify_type A in
+                let B' := reify_type B in
+                constr:(tpArr A' B')
+  | nat => constr:(tpNat)
+  | interp_type ?A => constr:(A)
+  | _ => fail "" T "is not a type"
+  end.
+
+Lemma ack'_reification_helper: exists res,
+    interp_term nil res
+    = existT _ (tpArr tpNat (tpArr tpNat (tpArr tpNat tpNat))) ack'.
+Proof.
+  eexists.
+  unfold ack'.
+
+  repeat lazymatch goal with
+  | |- interp_term ?e ?t = existT _ ?T (fun _ => _) =>
+    eapply interp_tLam; intros ?
+  | |- interp_term ?e ?t = existT _ ?T O =>
+    eapply interp_tO
+  | |- interp_term ?e ?t = existT _ ?T S =>
+    eapply interp_tS
+  | |- interp_term ?e ?t = existT _ ?T Nat.recursion =>
+    eapply interp_tNatRec
+  | |- interp_term ?e ?t = existT _ ?B (?f ?a) =>
+    let A := type of a in
+    let A := eval cbv beta iota in A in
+    let A := reify_type A in
+    eapply (interp_tApp e _ _ A B)
+  | |- interp_term ?e ?t = existT _ ?T ?x =>
+    is_var x;
+    first [eapply interp_tVar_head | eapply interp_tVar_tail]
+  end.
+
+Abort.
+
+
 Definition contender_5: nat. Admitted.
 
 
